@prefix rdf: <http://www.w3.org/1999/02/22-rdf-syntax-ns#> .
@prefix owl: <http://www.w3.org/2002/07/owl#> .
@prefix dcterms: <http://purl.org/dc/terms/> .
@prefix xsd: <http://www.w3.org/2001/XMLSchema#> .
@prefix vann: <http://purl.org/vocab/vann/> .
@prefix foaf: <http://xmlns.com/foaf/0.1/> .
@prefix dc: <http://purl.org/dc/elements/1.1/> .
@prefix void: <http://rdfs.org/ns/void#> .
@prefix rdfs: <http://www.w3.org/2000/01/rdf-schema#> .
@prefix formats: <http://www.w3.org/ns/formats/> .
@prefix void-ext: <http://ldf.fi/void-ext#> .

<http://ldf.fi/void-ext> a owl:Ontology ;
	owl:versionInfo "1.0.0" ;
	owl:imports <http://rdfs.org/ns/void> ;
	dcterms:title "Extensions to the Vocabulary of Interlinked Datasets (VoID)" ;
	dcterms:description "Extensions to the Vocabulary of Interlinked Datasets (VoID)" ;
	dcterms:modified "2014-02-17"^^xsd:date ;
	foaf:homepage <http://ldf.fi/schema/void-ext/index.html> ;
	vann:preferredNamespaceUri "http://ldf.fi/void-ext#";
    	vann:preferredNamespacePrefix "void-ext";
	dcterms:created "2014-02-17"^^xsd:date ;
	dcterms:publisher "Semantic Computing Research Group" ;
	dc:creator "Eetu Mäkelä" .

void-ext:distinctRDFNodes
	a owl:DatatypeProperty ;
	rdfs:label "distinct RDF nodes" ;
	rdfs:comment "The total number of distinct RDF nodes in a void:Dataset. In other words, the number of distinct literals, IRI references and blank nodes that occur in the subject, predicate or object position of triples in the dataset." ;
	rdfs:domain void:Dataset ;
	rdfs:range xsd:integer .

void-ext:distinctIRIReferences
	a owl:DatatypeProperty ;
	rdfs:label "distinct IRI references" ;
	rdfs:comment "The total number of distinct IRI references in a void:Dataset. In other words, the number of distinct IRI references that occur in the subject, predicate or object position of triples in the dataset." ;
	rdfs:domain void:Dataset ;
	rdfs:range xsd:integer .

void-ext:distinctBlankNodes
	a owl:DatatypeProperty ;
	rdfs:label "distinct blank nodes" ;
	rdfs:comment "The total number of distinct blank nodes in a void:Dataset. In other words, the number of distinct blank nodes that occur in the subject or object position of triples in the dataset." ;
	rdfs:domain void:Dataset ;
	rdfs:range xsd:integer .

void-ext:distinctLiterals
	a owl:DatatypeProperty ;
	rdfs:label "distinct literals" ;
	rdfs:comment "The total number of distinct literals in a void:Dataset. In other words, the number of distinct literals that occur in the object position of triples in the dataset." ;
	rdfs:domain void:Dataset ;
	rdfs:range xsd:integer .

void-ext:distinctIRIReferenceSubjects
	a owl:DatatypeProperty ;
	rdfs:label "distinct IRI reference subjects" ;
	rdfs:comment "The total number of distinct IRI reference subjects in a void:Dataset. In other words, the number of distinct IRI references that occur in the subject position of triples in the dataset." ;
	rdfs:domain void:Dataset ;
	rdfs:range xsd:integer .

void-ext:distinctBlankNodeSubjects
	a owl:DatatypeProperty ;
	rdfs:label "distinct blank node subjects" ;
	rdfs:comment "The total number of distinct blank node subjects in a void:Dataset. In other words, the number of distinct blank nodes that occur in the subject position of triples in the dataset." ;
	rdfs:domain void:Dataset ;
	rdfs:range xsd:integer .

void-ext:distinctIRIReferenceObjects
	a owl:DatatypeProperty ;
	rdfs:label "distinct IRI reference objects" ;
	rdfs:comment "The total number of distinct IRI reference objects in a void:Dataset. In other words, the number of distinct IRI references that occur in the object position of triples in the dataset." ;
	rdfs:domain void:Dataset ;
	rdfs:range xsd:integer .

void-ext:distinctBlankNodeObjects
	a owl:DatatypeProperty ;
	rdfs:label "distinct blank node objects" ;
	rdfs:comment "The total number of distinct blank node objects in a void:Dataset.  In other words, the number of distinct blank nodes that occur in the object position of triples in the dataset." ;
	rdfs:domain void:Dataset ;
	rdfs:range xsd:integer .

void-ext:propertyClasses 
	a owl:DatatypeProperty ;
	rdfs:label "property classes";
	rdfs:comment "The total number of distinct property classes in a void:Dataset. In other words, the number of distinct resources occuring as objects of rdf:type triples in the dataset, where the subjects of the rdf:type triples occur in the predicate position of triples in the dataset." ;
	rdfs:domain void:Dataset ;
	rdfs:range xsd:integer .

void-ext:objectClasses 
	a owl:DatatypeProperty ;
	rdfs:label "object classes";
	rdfs:comment "The total number of distinct object classes in a void:Dataset. In other words, the number of distinct resources occuring as objects of rdf:type triples in the dataset, where the subjects of the rdf:type triples occur in the object position of triples in the dataset." ;
	rdfs:domain void:Dataset ;
	rdfs:range xsd:integer .

void-ext:datatypes
	a owl:DatatypeProperty ;
	rdfs:label "datatypes" ;
	rdfs:comment "The total number of literal datatypes in a void:Dataset. In other words, the number of distinct datatypes that appear in any datatyped literal objects in the dataset." ;
	rdfs:domain void:Dataset ;
	rdfs:range xsd:integer .

void-ext:languages
	a owl:DatatypeProperty ;
	rdfs:label "languages" ;
	rdfs:comment "The total number of literal languages in a void:Dataset. In other words, the number of distinct languages that appear in any language literal objects in the dataset." ;
	rdfs:domain void:Dataset ;
	rdfs:range xsd:integer .

void-ext:subjectPartition
	a owl:ObjectProperty ;
	rdfs:label "subject partition" ;
	rdfs:comment "A subset of a void:Dataset that contains only triples with a certain subject." ;
	rdfs:domain void:Dataset ;
	rdfs:range void:Dataset ;
	rdfs:subPropertyOf void:subset .

void-ext:subject
	a owl:ObjectProperty, owl:FunctionalProperty ;
	rdfs:label "subject" ;
	rdfs:comment "the resource that is the subject of all triples in a subject-based partition." ;
	rdfs:domain void:Dataset ;
	rdfs:range rdfs:Resource .

void-ext:objectPartition
	a owl:ObjectProperty ;
	rdfs:label "object partition" ;
	rdfs:comment "A subset of a void:Dataset that contains only triples with a certain object." ;
	rdfs:domain void:Dataset ;
	rdfs:range void:Dataset ;
	rdfs:subPropertyOf void:subset .

void-ext:object
	a rdf:Property, owl:FunctionalProperty ;
	rdfs:label "object" ;
	rdfs:comment "the resource that is the object of all triples in an object-based partition." ;
	rdfs:domain void:Dataset ;
	rdfs:range rdfs:Resource .

void-ext:subjectNamespacePartition
	a owl:ObjectProperty ;
	rdfs:label "subject namespace partition" ;
	rdfs:comment "A subset of a void:Dataset that contains only entities that occur in the subject position of triples in the dataset and start with a certain namespace." ;
	rdfs:domain void:Dataset ;
	rdfs:range void:Dataset ;
	rdfs:subPropertyOf void:subset .

void-ext:propertyNamespacePartition
	a owl:ObjectProperty ;
	rdfs:label "property namespace partition" ;
	rdfs:comment "A subset of a void:Dataset that contains only entities that occur in the predicate position of triples in the dataset and start with a certain namespace." ;
	rdfs:domain void:Dataset ;
	rdfs:range void:Dataset ;
	rdfs:subPropertyOf void:subset .

void-ext:objectNamespacePartition
	a owl:ObjectProperty ;
	rdfs:label "object namespace partition" ;
	rdfs:comment "A subset of a void:Dataset that contains only entities that occur in the object position of triples in the dataset and start with a certain namespace." ;
	rdfs:domain void:Dataset ;
	rdfs:range void:Dataset ;
	rdfs:subPropertyOf void:subset .

void-ext:namespace
	a owl:ObjectProperty, owl:FunctionalProperty ;
	rdfs:label "object" ;
	rdfs:comment "the namespace that is required of resources to be included into a namespace-based partition." ;
	rdfs:domain void:Dataset ;
	rdfs:range rdfs:Resource .

void-ext:propertyClassPartition
	a owl:ObjectProperty ;
	rdfs:label "property class partition" ;
	rdfs:comment "A subset of a void:Dataset that contains only entities of a certain rdfs:Class that occur in the predicate position of triples in the dataset." ;
	rdfs:domain void:Dataset ;
	rdfs:range void:Dataset ;
	rdfs:subPropertyOf void:subset .

void-ext:objectClassPartition
	a owl:ObjectProperty ;
	rdfs:label "object class partition" ;
	rdfs:comment "A subset of a void:Dataset that contains only entities of a certain rdfs:Class that occur in the object position of triples in the dataset." ;
	rdfs:domain void:Dataset ;
	rdfs:range void:Dataset ;
	rdfs:subPropertyOf void:subset .

